\include{"../preamble.tex"}
\title{ECE 113 HW 2}
\begin{document}
\maketitle
\section*{Problem 1}
\subsection*{(a)}
The discrete fourier transform doesn't exist since we have
\begin{align*}
    X(\omega)&=\sum_{n=-\infty}^\infty x[n]e^{-j\omega n}\\
    &=\sum_{n=0}^{2\frac{1}{\omega}-1}3^{n}e^{-j\omega n}\sum_{k=-\infty}^{\infty}3^{\frac{2k}{\omega}}
\end{align*}
Since this second sum does not converge since $3>1$, this means that
the DTFT doesn't exist.
\subsection*{(b)}
\subsubsection*{(i)}
This DTFT doesn't exist since once again we can write the fourier transform
as 
$$X(\omega)=\sum_{n=0}^{2\frac{1}{\omega}-1}3^{n}e^{-j\omega n}\sum_{k=0}^{\infty}3^{\frac{2k}{\omega}}$$
And once again this second sum does not converge since $3>1$.
\subsubsection*{(ii)}
This does exist, since we can write 
$$X[-n]u[n]=3^{-n}u[n]$$
Whose fourier transform is 
$$3^{-n}u[n]\to \frac{1}{1-\frac{e^{-j\omega}}{3}}$$
\subsubsection*{(iii)}
$$x[|n|]=x[-n]u[n]+x[n]u[-n]$$
from the time reversal property we have that
$$x[-n]u[n]+x[n]u[-n]\to \frac{1}{1-\frac{e^{-j\omega}}{3}}+\frac{1}{1-\frac{e^{j\omega}}{3}}$$
\subsubsection*{(iv)}
From the time reversal property we have that
$$x[n]u[-n]\to\frac{1}{1-\frac{e^{j\omega}}{3}}$$
\section*{Problem 2}
\subsection*{(a)}
We have that 
$$\sin(\Omega_0n)=\frac{1}{2j}\left(e^{j\Omega_0n}-e^{-j\Omega_0n}\right)$$
And so we have that 
$$X(\Omega)=\frac{\pi}{j}\left(\delta(\Omega-\Omega_0)-\delta(\Omega+\Omega_0)\right)$$
\subsection*{(b)}
We have that
$$|X(\Omega)|=\pi\left(\delta(\Omega-\Omega_0)+\delta(\Omega+\Omega_0)\right)$$
and 
$$\angle X(\Omega)=\frac{\pi}{2}\left(\delta(\Omega-\Omega_0)-\delta(\Omega+\Omega_0)\right)$$
\section*{Problem 3}
\subsection*{(a)}
$$\tilde{x}[n]\bigotimes\tilde{x}[n]=[3, 3, 3, 4, 3]$$
\subsection*{(b)}
$$\tilde{x}[n]\bigotimes \tilde{y}[n]=[0, 0, 0, 0, 0, 0]$$
\section*{Problem 4}
We have that 
\begin{align*}
    x[n]\cos(\Omega_0 n)&=\frac{x[n]}{2}\left(e^{j\Omega_0 n}+e^{-j\Omega_0 n}\right)\\
    &\to \frac{1}{2}\left(X(\Omega-\Omega_0)+X(\Omega+\Omega_0)\right)
\end{align*}
\section*{Problem 5}
We have that taking the fourier transform of the diffrence equation
$$Y(\omega)(1+\frac{4}{9}e^{-j\omega}+\frac{1}{27}e^{-2j\omega})=X(\omega)(1-\frac{8}{9}e^{-j\omega}+\frac{1}{3}e^{-2j\omega})$$
Since $x[n]$ is the delta function we have that 
$X(\omega)=1$ and thus we have
\begin{align*}
    Y(\omega)&=\frac{3(9-8e^{-j\omega}-3e^{-2j\omega})}{(3+e^{-j\omega})(9+e^{-j\omega})}\\
    &=3\left(\frac{1}{3+e^{-j\omega}}-\frac{3e^{-j\omega}}{9+e^{-j\omega}}\right)\\
    &\to \boxed{(-3)^{n}u[n]-(-9)^{n-1}u[n-1]}
\end{align*}
\end{document}