\include{"../preamble.tex"}
\title{ECE 113 HW 2}
\begin{document}
\maketitle
\section*{Problem 1}
We have that 
$$h[-n]=\{4,-6,5-3\},-1\leq n \leq 2$$
Thus 
$$h[-n-1]=\{4,-6,5-3\},-2\leq n \leq 1$$
So $y[-1]=-12-15-12=\boxed{-39}$
\section*{Problem 2}
\subsection*{(a)}
$$x_1[n]*x_1[n]=\boxed{\{1,-2,3,-2,1\},-2\leq n \leq 2}$$
\subsection*{(b)}
$$x_2[n]*x_2[n]=\boxed{\{1,-2,1,2,-4,2,1,-2,1\},0\leq n \leq 8}$$
\subsection*{(c)}
$$x_3[n]*x_3[n]=\boxed{\{1, -4, 4, 4, -10, 4, 4, -4, 1\},-6\leq n \leq 2}$$
\section*{Problem 3}
We have that the output $y[n]$ is 
\begin{align*}
y[n]&=h[n]*x[n]\\
&=\sum_{k=-\infty}^{\infty}h[k]x[n-k]\\
&=\sum_{k=-\infty}^{\infty}2^{k}u[k]2^{-(n-k)}u[n-k]
\end{align*}
Therefore in the case that $n<0$ we have
\begin{align*}
y[n]&=\sum_{k=-\infty}^{n}2^{2k-n}\\
y[n]&=2^{-n}\sum_{j=-n}^{\infty}2^{-2j}\\
y[n]=2^{n}\sum_{i=0}^{\infty}2^{-2i}\\
y[n]&=2^{n}\frac{1}{1-2^{-2}}\\
y[n]&=2^{n+2}\frac{1}{3}
\end{align*}
In the case that $n\geq 0$ we have
\begin{align*}
y[n]&=\sum_{k=-\infty}^{0}2^{2k-n}\\
&=2^{-n}\sum_{j=0}^{\infty}2^{-2j}\\
&=2^{-n}\frac{1}{1-2^{-2}}\\
&=2^{-n+2}\frac{1}{3}
\end{align*}
Therefore we have
$$y[n]=\boxed{\begin{cases}
2^{n+2}\frac{1}{3} & n<0\\
2^{-n+2}\frac{1}{3} & n\geq 0
\end{cases}}$$
\section*{Problem 4}
\subsection*{(a)}
$$x[n]*y[n]=\boxed{\{3,5,6,7,7,8,9,9,7,4,2,1\},-3\leq n \leq 8}$$
\subsection*{(b)}
Then the response $y_2[n]$ would be 
\begin{align*}
y_2[n]=&h_1[n]*\left(\left(\frac{1}{3}\right)^nu[n]\right)\\
=&\frac{1}{2^{n+1}}x[n+2]u[n]*\left(\left(\frac{1}{3}\right)^nu[n]\right)-\frac{3}{2}
\delta[n]u[n]*\left(\left(\frac{1}{3}\right)^nu[n]\right)\\
&+\frac{1}{2^n}u[n-3]u[n]*\left(\left(\frac{1}{3}\right)^nu[n]\right)\\
\end{align*}
We have that $x[n+2]*\left(\left(\frac{1}{3}\right)^nu[n]\right)=0$ 
if $n<0$ and for $n\geq 0$ we have:
\begin{align*}
    \frac{1}{2^(n+1)}x[n+2]u[n]*\left(\left(\frac{1}{3}\right)^nu[n]\right)&=\sum_{k=-\infty}^{\infty}\frac{1}{2^{(k+1)}}x[k+2]u[k]\left(\left(\frac{1}{3}\right)^{n-k}u[n-k]\right)\\
    &=\left(\frac{1}{3}\right)^n\sum_{k=0}^{n}2^{-k-1} 3^{k}x[k+2]
\end{align*}
Likewise we have that $\delta[n]*\left(\left(\frac{1}{3}\right)^nu[n]\right)=\left(\frac{1}{3}\right)^nu[n]$, and 
for $ \left(2^{-n}u[n-3]\right)*\left(3^{-n}u[n]\right)$ we get that for $n<3$ the sequence is $0$ and otherwise we have
\begin{align*}
    \left(2^{-n}u[n-3]\right)*\left(3^{-n}u[n]\right)&=\sum_{k=-\infty}^{\infty}2^{-k}u[k-3]3^{-k+n}u[n-k]\\
    &=\sum_{k=3}^{n}2^{-k}3^{k-n}\\
    &=3^{-n}\sum_{k=3}^{n}\left(\frac{3}{2}\right)^{k}\\
    &=3^{-n}2\left(\left(\frac{3}{2}\right)^n-\left(\frac{3}{2}\right)^2\right)
\end{align*}
Therefore we have that 
$$y_2[n]=\boxed{\begin{cases}
    0 & n<0\\
    -\frac{3}{2}\left(\frac{1}{3}\right)^n+3^{-n}\sum_{k=0}^{n}2^{-k-1} 3^{k}x[k+2] & 0\leq n<3\\
    -\frac{3}{2}\left(\frac{1}{3}\right)^n+3^{-n}2\left(\left(\frac{3}{2}\right)^n-\left(\frac{3}{2}\right)^2\right)+3^{-n}\sum_{k=0}^{4}2^{-k-1} 3^{k}x[k+2] & n\geq 3
\end{cases}}$$
\section*{Problem 5}
\subsection*{(a)}
The first index is the index $n$ that satisfies the condition 
$n-n_1-n_3=0$, thus we get that the first nonzero element occurs at $\boxed{n_1+n_3}$
\subsection*{(b)}
The last index is the index $n$ that satisfies the condition
$n-(n_2-1)-(n_4-1)=0$, thus we get that the last nonzero element occurs at $\boxed{n_2+n_4-2}$
\subsection*{(c)}
Therefore the length of the output sequence is 
$n_2+n_4-2-(n_1+n_3)+1=\boxed{n_x+n_h-1}$






\end{document}